
\documentclass[12pt]{amsart}
\usepackage{geometry} % see geometry.pdf on how to lay out the page. There's lots.
\usepackage{amssymb}
\geometry{a4paper} % or letter or a5paper or ... etc
% \geometry{landscape} % rotated page geometry

% See the ``Article customise'' template for come common customisations

\title{}
\author{}
\date{} % delete this line to display the current date

\newcommand{\fhat}{\frac{1}{h}\int_{x-(h/2)}^{x+(h/2)}f(y)dy}

%%% BEGIN DOCUMENT
\begin{document}

\maketitle

Let $\lambda$=log($\frac{\pi}{1-\pi}$). 

$$
e^{\lambda y - \psi(\lambda)} = AB 
$$

where 

$$
A = {(\frac{\pi}{1-\pi})}^y
$$

and 

$$
B = (1 + \frac{\pi}{1-\pi})^{-n}
$$

So we have 

$$
AB = \frac{{(\frac{\pi}{1-\pi})}^y }{ (1 + \frac{\pi}{1-\pi})^{n}}
$$

Splitting the exponent we have

\begin{equation}
AB = \frac{{(\frac{\pi}{1-\pi})}^y }{ (1 + \frac{\pi}{1-\pi})(1 + \frac{\pi}{1-\pi})^{n-1}} 
\end{equation}

Multiplying $AB$ by $\frac{1-\pi}{1-\pi}=1$

\begin{equation}
AB = \frac{{\frac{\pi^y}{(1-\pi)^y}} (1-\pi)}{ ({1-\pi} + \pi)(1 + \frac{\pi}{1-\pi})^{n-1}}
\end{equation}

\begin{equation}
AB = \frac{{\frac{\pi^y}{(1-\pi)^{y-1}}}}{(1 + \frac{\pi}{1-\pi})^{n-1}}
\end{equation}

If we repeat (1), (2) and (3) $n$ times we have 

$$
AB = \frac{{\frac{\pi^y}{(1-\pi)^{y-n}}}}{(1 + \frac{\pi}{1-\pi})^{n-n}}
$$

$$
AB = {\frac{\pi^y}{(1-\pi)^{y-n}}}
$$

$$
AB = \pi^y (1-\pi)^{(-(y-n)}
$$

$$
AB = \pi^y (1-\pi)^{n-y}
$$

\end{document}